src/cbor/pulse/raw/everparse/CBOR.Pulse.Raw.EverParse.Insert.fsti
@@ -1,0 +1,78 @@
+module CBOR.Pulse.Raw.EverParse.Insert
+
+open CBOR.Spec.Raw.EverParse
+open CBOR.Spec.Raw.Format
+open CBOR.Spec.Raw.Base
+open Pulse.Lib.Pervasives
+open Pulse.Lib.Slice
+
+module S = Pulse.Lib.Slice
+module SZ = FStar.SizeT
+module U8 = FStar.UInt8
+
+val cbor_raw_map_insert_out_inv
+  (off1: SZ.t)
+  (m: list (raw_data_item & raw_data_item))
+  (off2: SZ.t)
+  (key: raw_data_item)
+  (off3: SZ.t)
+  (value: raw_data_item)
+  (v: Seq.seq U8.t)
+: Tot prop
+
+val cbor_raw_map_insert_out_inv_intro
+  (off1: SZ.t)
+  (m: list (raw_data_item & raw_data_item))
+  (off2: SZ.t)
+  (key: raw_data_item)
+  (off3: SZ.t)
+  (value: raw_data_item)
+  (v: Seq.seq U8.t)
+: Lemma
+  (requires (
+    let sm = serialize_cbor_map m in
+    let sk = serialize_cbor key in
+    let sv = serialize_cbor value in
+    SZ.v off1 + Seq.length sm == SZ.v off2 /\
+    SZ.v off2 + Seq.length sk == SZ.v off3 /\
+    SZ.v off3 + Seq.length sv == Seq.length v /\
+    Seq.slice v (SZ.v off1) (SZ.v off2) `Seq.equal` sm /\
+    Seq.slice v (SZ.v off2) (SZ.v off3) `Seq.equal` sk /\
+    Seq.slice v (SZ.v off3) (Seq.length v) `Seq.equal` sv
+  ))
+  (ensures (cbor_raw_map_insert_out_inv off1 m off2 key off3 value v))
+
+val cbor_raw_map_insert_post
+  (m: list (raw_data_item & raw_data_item))
+  (key: raw_data_item)
+  (value: raw_data_item)
+  (res: bool)
+  (v': Seq.seq U8.t)
+: Tot prop
+
+val cbor_raw_map_insert_post_elim
+  (m: list (raw_data_item & raw_data_item))
+  (key: raw_data_item)
+  (value: raw_data_item)
+  (res: bool)
+  (v': Seq.seq U8.t)
+: Lemma
+  (requires (cbor_raw_map_insert_post m key value res v'))
+  (ensures (
+    match cbor_map_insert m (key, value) with
+    | None -> res == false
+    | Some m' -> res == true /\ v' == serialize_cbor_map m'
+  ))
+
+val cbor_raw_map_insert
+  (out: S.slice U8.t)
+  (m: Ghost.erased (list (raw_data_item & raw_data_item)))
+  (off2: SZ.t)
+  (key: Ghost.erased raw_data_item)
+  (off3: SZ.t)
+  (value: Ghost.erased raw_data_item)
+  (#v: Ghost.erased (Seq.seq U8.t))
+: stt bool
+    (pts_to out v ** pure (cbor_raw_map_insert_out_inv 0sz m off2 key off3 value v))
+    (fun res -> exists* v' . pts_to out v' **
+      pure (cbor_raw_map_insert_post m key value res v'))
